examples/programs/vstte12_ring_buffer_2/vstte12_ring_buffer_2_RingBuffer_WP_parameter_head_1.v
@@ -25,11 +25,9 @@ Existing Instance option_WhyType.
 Implicit Arguments None [[a] [a_WT]].
 Implicit Arguments Some [[a] [a_WT]].
 
-Parameter nth: forall {a:Type} {a_WT:WhyType a}, BuiltIn.int -> (list a) ->
-  (option a).
+Parameter nth: forall {a:Type} {a_WT:WhyType a}, Z -> (list a) -> (option a).
 
-Axiom nth_def : forall {a:Type} {a_WT:WhyType a}, forall (n:BuiltIn.int)
-  (l:(list a)),
+Axiom nth_def : forall {a:Type} {a_WT:WhyType a}, forall (n:Z) (l:(list a)),
   match l with
   | Nil => ((nth n l) = (None :(option a)))
   | (Cons x r) => ((n = 0%Z) -> ((nth n l) = (Some x))) /\ ((~ (n = 0%Z)) ->
@@ -37,8 +35,7 @@ Axiom nth_def : forall {a:Type} {a_WT:WhyType a}, forall (n:BuiltIn.int)
   end.
 
 (* Why3 assumption *)
-Fixpoint length {a:Type} {a_WT:WhyType a}(l:(list
-  a)) {struct l}: BuiltIn.int :=
+Fixpoint length {a:Type} {a_WT:WhyType a}(l:(list a)) {struct l}: Z :=
   match l with
   | Nil => 0%Z
   | (Cons _ r) => (1%Z + (length r))%Z
@@ -51,13 +48,13 @@ Axiom Length_nil : forall {a:Type} {a_WT:WhyType a}, forall (l:(list a)),
   ((length l) = 0%Z) <-> (l = (Nil :(list a))).
 
 Axiom nth_none_1 : forall {a:Type} {a_WT:WhyType a}, forall (l:(list a))
-  (i:BuiltIn.int), (i < 0%Z)%Z -> ((nth i l) = (None :(option a))).
+  (i:Z), (i < 0%Z)%Z -> ((nth i l) = (None :(option a))).
 
 Axiom nth_none_2 : forall {a:Type} {a_WT:WhyType a}, forall (l:(list a))
-  (i:BuiltIn.int), ((length l) <= i)%Z -> ((nth i l) = (None :(option a))).
+  (i:Z), ((length l) <= i)%Z -> ((nth i l) = (None :(option a))).
 
 Axiom nth_none_3 : forall {a:Type} {a_WT:WhyType a}, forall (l:(list a))
-  (i:BuiltIn.int), ((nth i l) = (None :(option a))) -> ((i < 0%Z)%Z \/
+  (i:Z), ((nth i l) = (None :(option a))) -> ((i < 0%Z)%Z \/
   ((length l) <= i)%Z).
 
 (* Why3 assumption *)
@@ -95,16 +92,15 @@ Axiom mem_decomp : forall {a:Type} {a_WT:WhyType a}, forall (x:a) (l:(list
   (l = (infix_plpl l1 (Cons x l2))).
 
 Axiom nth_append_1 : forall {a:Type} {a_WT:WhyType a}, forall (l1:(list a))
-  (l2:(list a)) (i:BuiltIn.int), (i < (length l1))%Z -> ((nth i
-  (infix_plpl l1 l2)) = (nth i l1)).
+  (l2:(list a)) (i:Z), (i < (length l1))%Z -> ((nth i (infix_plpl l1
+  l2)) = (nth i l1)).
 
 Axiom nth_append_2 : forall {a:Type} {a_WT:WhyType a}, forall (l1:(list a))
-  (l2:(list a)) (i:BuiltIn.int), ((length l1) <= i)%Z -> ((nth i
-  (infix_plpl l1 l2)) = (nth (i - (length l1))%Z l2)).
+  (l2:(list a)) (i:Z), ((length l1) <= i)%Z -> ((nth i (infix_plpl l1
+  l2)) = (nth (i - (length l1))%Z l2)).
 
-Parameter map : forall (a:Type) {a_WT:WhyType a} (b:Type) {b_WT:WhyType b},
-  Type.
-Axiom map_WhyType : forall (a:Type) {a_WT:WhyType a}
+Axiom map : forall (a:Type) {a_WT:WhyType a} (b:Type) {b_WT:WhyType b}, Type.
+Parameter map_WhyType : forall (a:Type) {a_WT:WhyType a}
   (b:Type) {b_WT:WhyType b}, WhyType (map a b).
 Existing Instance map_WhyType.
 
@@ -130,35 +126,38 @@ Axiom Const : forall {a:Type} {a_WT:WhyType a} {b:Type} {b_WT:WhyType b},
 
 (* Why3 assumption *)
 Inductive array (a:Type) {a_WT:WhyType a} :=
-  | mk_array : BuiltIn.int -> (map BuiltIn.int a) -> array a.
+  | mk_array : Z -> (map Z a) -> array a.
 Axiom array_WhyType : forall (a:Type) {a_WT:WhyType a}, WhyType (array a).
 Existing Instance array_WhyType.
 Implicit Arguments mk_array [[a] [a_WT]].
 
 (* Why3 assumption *)
-Definition elts {a:Type} {a_WT:WhyType a}(v:(array a)): (map BuiltIn.int
-  a) := match v with
+Definition elts {a:Type} {a_WT:WhyType a}(v:(array a)): (map Z a) :=
+  match v with
   | (mk_array x x1) => x1
   end.
 
 (* Why3 assumption *)
-Definition length1 {a:Type} {a_WT:WhyType a}(v:(array a)): BuiltIn.int :=
+Definition length1 {a:Type} {a_WT:WhyType a}(v:(array a)): Z :=
   match v with
   | (mk_array x x1) => x
   end.
 
 (* Why3 assumption *)
-Definition get1 {a:Type} {a_WT:WhyType a}(a1:(array a)) (i:BuiltIn.int): a :=
+Definition get1 {a:Type} {a_WT:WhyType a}(a1:(array a)) (i:Z): a :=
   (get (elts a1) i).
 
 (* Why3 assumption *)
-Definition set1 {a:Type} {a_WT:WhyType a}(a1:(array a)) (i:BuiltIn.int)
-  (v:a): (array a) := (mk_array (length1 a1) (set (elts a1) i v)).
+Definition set1 {a:Type} {a_WT:WhyType a}(a1:(array a)) (i:Z) (v:a): (array
+  a) := (mk_array (length1 a1) (set (elts a1) i v)).
+
+(* Why3 assumption *)
+Definition make {a:Type} {a_WT:WhyType a}(n:Z) (v:a): (array a) :=
+  (mk_array n (const v:(map Z a))).
 
 (* Why3 assumption *)
 Inductive buffer (a:Type) {a_WT:WhyType a} :=
-  | mk_buffer : BuiltIn.int -> BuiltIn.int -> (array a) -> (list
-      a) -> buffer a.
+  | mk_buffer : Z -> Z -> (array a) -> (list a) -> buffer a.
 Axiom buffer_WhyType : forall (a:Type) {a_WT:WhyType a}, WhyType (buffer a).
 Existing Instance buffer_WhyType.
 Implicit Arguments mk_buffer [[a] [a_WT]].
@@ -176,39 +175,38 @@ Definition data {a:Type} {a_WT:WhyType a}(v:(buffer a)): (array a) :=
   end.
 
 (* Why3 assumption *)
-Definition len {a:Type} {a_WT:WhyType a}(v:(buffer a)): BuiltIn.int :=
+Definition len {a:Type} {a_WT:WhyType a}(v:(buffer a)): Z :=
   match v with
   | (mk_buffer x x1 x2 x3) => x1
   end.
 
 (* Why3 assumption *)
-Definition first {a:Type} {a_WT:WhyType a}(v:(buffer a)): BuiltIn.int :=
+Definition first {a:Type} {a_WT:WhyType a}(v:(buffer a)): Z :=
   match v with
   | (mk_buffer x x1 x2 x3) => x
   end.
 
 (* Why3 assumption *)
-Definition size {a:Type} {a_WT:WhyType a}(b:(buffer a)): BuiltIn.int :=
+Definition size {a:Type} {a_WT:WhyType a}(b:(buffer a)): Z :=
   (length1 (data b)).
 
 Require Import Why3.
 Ltac ae := why3 "alt-ergo" timelimit 3.
 
 (* Why3 goal *)
-Theorem WP_parameter_head : forall {a:Type} {a_WT:WhyType a},
-  forall (b:BuiltIn.int), forall (rho:(list a)) (rho1:(map BuiltIn.int a))
-  (rho2:BuiltIn.int) (rho3:BuiltIn.int), ((0%Z < rho2)%Z /\
-  (((0%Z <= rho3)%Z /\ (rho3 < b)%Z) /\ (((0%Z <= rho2)%Z /\
-  (rho2 <= b)%Z) /\ ((rho2 = (length rho)) /\ forall (i:BuiltIn.int),
-  ((0%Z <= i)%Z /\ (i < rho2)%Z) -> ((((rho3 + i)%Z < b)%Z -> ((nth i
-  rho) = (Some (get rho1 (rho3 + i)%Z)))) /\
-  ((0%Z <= ((rho3 + i)%Z - b)%Z)%Z -> ((nth i rho) = (Some (get rho1
-  ((rho3 + i)%Z - b)%Z))))))))) -> (((0%Z <= rho3)%Z /\ (rho3 < b)%Z) ->
+Theorem WP_parameter_head : forall {a:Type} {a_WT:WhyType a}, forall (b:Z),
+  forall (rho:(list a)) (rho1:(map Z a)) (rho2:Z) (rho3:Z),
+  ((((0%Z <= rho3)%Z /\ (rho3 < b)%Z) /\ (((0%Z <= rho2)%Z /\
+  (rho2 <= b)%Z) /\ ((rho2 = (length rho)) /\ forall (i:Z), ((0%Z <= i)%Z /\
+  (i < rho2)%Z) -> ((((rho3 + i)%Z < b)%Z -> ((nth i rho) = (Some (get rho1
+  (rho3 + i)%Z)))) /\ ((0%Z <= ((rho3 + i)%Z - b)%Z)%Z -> ((nth i
+  rho) = (Some (get rho1 ((rho3 + i)%Z - b)%Z)))))))) /\ (0%Z < rho2)%Z) ->
+  (((0%Z <= rho3)%Z /\ (rho3 < b)%Z) ->
   match rho with
   | Nil => False
   | (Cons x _) => ((get rho1 rho3) = x)
   end).
-intros a _a b rho rho1 rho2 rho3 (h1,(h2,(h2b,(h2c,h2d)))) (h3,h4).
+intros a _a b rho rho1 rho2 rho3 ((h2,(h2b,(h2c,h2d))),h1) (h3,h4).
 destruct rho.
 simpl in *.
 omega.
